removed legacy ML files;

src/HOL/Modelcheck/MuckeSyn.thy
@@ -71,6 +71,176 @@ syntax (Mucke output)
 oracle mc_mucke_oracle ("term") =
   mk_mc_mucke_oracle
 
+ML {*
+(* search_mu t searches for Mu terms in term t. In the case of nested Mu's,
+   it yields innermost one. If no Mu term is present, search_mu yields NONE
+*)
+
+(* extended for treatment of nu (TH) *)
+fun search_mu ((Const("MuCalculus.mu",tp)) $ t2) = 
+	(case (search_mu t2) of
+	      SOME t => SOME t 
+	    | NONE => SOME ((Const("MuCalculus.mu",tp)) $ t2))
+  | search_mu ((Const("MuCalculus.nu",tp)) $ t2) =
+        (case (search_mu t2) of
+              SOME t => SOME t
+            | NONE => SOME ((Const("MuCalculus.nu",tp)) $ t2))
+  | search_mu (t1 $ t2) = 
+	(case (search_mu t1) of
+	      SOME t => SOME t 
+	    | NONE     => search_mu t2)
+  | search_mu (Abs(_,_,t)) = search_mu t
+  | search_mu _ = NONE;
+
+
+
+
+(* seraching a variable in a term. Used in move_mus to extract the
+   term-rep of var b in hthm *)
+
+fun search_var s t =
+case t of
+     t1 $ t2 => (case (search_var s t1) of
+		             SOME tt => SOME tt |
+			     NONE => search_var s t2) |
+     Abs(_,_,t) => search_var s t |
+     Var((s1,_),_) => if s = s1 then SOME t else NONE |
+     _ => NONE;
+	
+
+(* function move_mus:
+   Mucke can't deal with nested Mu terms. move_mus i searches for 
+   Mu terms in the subgoal i and replaces Mu terms in the conclusion
+   by constants and definitions in the premises recursively.
+
+   move_thm is the theorem the performs the replacement. To create NEW
+   names for the Mu terms, the indizes of move_thm are incremented by
+   max_idx of the subgoal.
+*)
+
+local
+
+  val move_thm = prove_goal (the_context ()) "[| a = b ==> P a; a = b |] ==> P b"
+	(fn prems => [cut_facts_tac prems 1, dtac sym 1, hyp_subst_tac 1,
+		     REPEAT (resolve_tac prems 1)]);
+
+  val sig_move_thm = Thm.theory_of_thm move_thm;
+  val bCterm = cterm_of sig_move_thm (valOf (search_var "b" (concl_of move_thm)));
+  val aCterm = cterm_of sig_move_thm (valOf (search_var "a" (hd(prems_of move_thm)))); 
+
+in
+
+fun move_mus i state =
+let val sign = Thm.theory_of_thm state;
+    val (subgoal::_) = Library.drop(i-1,prems_of state);
+    val concl = Logic.strip_imp_concl subgoal; (* recursive mu's in prems? *)
+    val redex = search_mu concl;
+    val idx = let val t = #maxidx (rep_thm state) in 
+	      if t < 0 then 1 else t+1 end;
+in
+case redex of
+     NONE => all_tac state |
+     SOME redexterm => 
+	let val Credex = cterm_of sign redexterm;
+	    val aiCterm = 
+		cterm_of sig_move_thm (Logic.incr_indexes ([],idx) (term_of aCterm));
+	    val inst_move_thm = cterm_instantiate 
+				[(bCterm,Credex),(aCterm,aiCterm)] move_thm;
+	in
+            ((rtac inst_move_thm i) THEN (dtac eq_reflection i) 
+		THEN (move_mus i)) state
+	end
+end;
+end;
+
+
+fun call_mucke_tac i state =
+let val thy = Thm.theory_of_thm state;
+    val OraAss = mc_mucke_oracle thy (Logic.nth_prem (i, Thm.prop_of state))
+in 
+(cut_facts_tac [OraAss] i) state
+end;
+
+
+(* transforming fun-defs into lambda-defs *)
+
+val [eq] = goal CPure.thy "(!! x. f x == g x) ==> f == g";
+ by (rtac (extensional eq) 1);
+qed "ext_rl";
+
+infix cc;
+
+fun NONE cc xl = xl
+  | (SOME x) cc xl = x::xl;
+
+fun getargs ((x $ y) $ (Var ((z,_),_))) = getargs (x $ y) ^ " " ^z
+  | getargs (x $ (Var ((y,_),_))) = y;
+
+fun getfun ((x $ y) $ z) = getfun (x $ y)
+  | getfun (x $ _) = x;
+
+local
+
+fun delete_bold [] = []
+| delete_bold (x::xs) = if (is_prefix (op =) ("\^["::"["::"0"::"m"::[]) (x::xs))
+        then (let val (_::_::_::s) = xs in delete_bold s end)
+        else (if (is_prefix (op =) ("\^["::"["::"1"::"m"::[]) (x::xs))
+                then  (let val (_::_::_::s) = xs in delete_bold s end)
+                else (x::delete_bold xs));
+
+fun delete_bold_string s = implode(delete_bold (explode s));
+
+in
+
+(* extension with removing bold font (TH) *)
+fun mk_lam_def (_::_) _ _ = NONE  
+  | mk_lam_def [] ((Const("==",_) $ (Const _)) $ RHS) t = SOME t
+  | mk_lam_def [] ((Const("==",_) $ LHS) $ RHS) t = 
+    let val thy = theory_of_thm t;
+	val fnam = Sign.string_of_term thy (getfun LHS);
+	val rhs = Sign.string_of_term thy (freeze_thaw RHS)
+	val gl = delete_bold_string (fnam ^" == % " ^ (getargs LHS) ^" . " ^ rhs);
+    in
+	SOME (prove_goal thy gl (fn prems =>
+  		[(REPEAT (rtac ext_rl 1)), (rtac t 1) ]))
+    end
+| mk_lam_def [] _ t= NONE; 
+
+fun mk_lam_defs ([]:thm list) = ([]: thm list) 
+  | mk_lam_defs (t::l) = 
+      (mk_lam_def (prems_of t) (concl_of t) t) cc (mk_lam_defs l);
+
+end;
+
+
+(* first simplification, then model checking *)
+
+val pair_eta_expand = Thm.symmetric (mk_meta_eq (thm "split_eta"));
+
+val pair_eta_expand_proc =
+  Simplifier.simproc (the_context ()) "pair_eta_expand" ["f::'a*'b=>'c"]
+  (fn _ => fn _ => fn t => case t of Abs _ => SOME pair_eta_expand | _ => NONE);
+
+val Mucke_ss = simpset() addsimprocs [pair_eta_expand_proc] addsimps [Let_def];
+
+
+(* the interface *)
+
+fun mc_mucke_tac defs i state =
+  (case Library.drop (i - 1, Thm.prems_of state) of
+    [] => no_tac state
+  | subgoal :: _ =>
+      EVERY [
+        REPEAT (etac thin_rl i),
+        cut_facts_tac (mk_lam_defs defs) i,
+        full_simp_tac (Mucke_ss delsimps [not_iff,split_part]) i,
+        move_mus i, call_mucke_tac i,atac i,
+        REPEAT (rtac refl i)] state);
+
+(*check if user has mucke installed*)
+fun mucke_enabled () = getenv "MUCKE_HOME" <> "";
+fun if_mucke_enabled f x = if mucke_enabled () then f x else ();
+
+*}
+
 end
-
-
