src/HOL/Modelcheck/EindhovenSyn.thy
@@ -59,4 +59,25 @@ in
 end
 *}
 
+ML {*
+fun mc_eindhoven_tac i state = SUBGOAL (fn (goal, _) =>
+  let
+    val thy = Thm.theory_of_thm state;
+    val assertion = mc_eindhoven_oracle thy (Logic.strip_imp_concl goal);
+  in cut_facts_tac [assertion] i THEN atac i end) i state;
+
+val pair_eta_expand = Thm.symmetric (mk_meta_eq (thm "split_eta"));
+
+val pair_eta_expand_proc =
+  Simplifier.simproc (the_context ()) "pair_eta_expand" ["f::'a*'b=>'c"]
+  (fn _ => fn _ => fn t => case t of Abs _ => SOME pair_eta_expand | _ => NONE);
+
+val Eindhoven_ss =
+  simpset() addsimprocs [pair_eta_expand_proc] addsimps [Let_def];
+
+(*check if user has pmu installed*)
+fun eindhoven_enabled () = getenv "EINDHOVEN_HOME" <> "";
+fun if_eindhoven_enabled f x = if eindhoven_enabled () then f x else ();
+*}
+
 end
